src/prop/PFCertify.v
@@ -1,3 +1,5 @@
+Require Import RelationClasses.
+
 From sflib Require Import sflib.
 From Paco Require Import paco.
 
@@ -25,54 +27,102 @@ Require Import Thread.
 Section PFCertify.
   Variable lang: language.
 
-  Variant certify (reserved: OptTimeMap.t) (loc: Loc.t) (th: Thread.t lang): Prop :=
-    | certify_failure
-        pf e th1 th2
-        (STEPS: rtc (Thread.tau_step reserved) th th1)
-        (STEP_FAILURE: Thread.step reserved pf e th1 th2)
-        (EVENT_FAILURE: ThreadEvent.get_machine_event e = MachineEvent.failure)
-    | certify_fulfill
-        pf e th1 th2
-        from to val released ord
-        (STEPS: rtc (Thread.tau_step reserved) th th1)
-        (STEP_FULFILL: Thread.step reserved pf e th1 th2)
-        (EVENT_FULFILL: ThreadEvent.is_writing e = Some (loc, from, to, val, released, ord))
-        (TO: Time.lt (Memory.max_ts loc (Global.memory (Thread.global th1))) to)
-        (ORD: Ordering.le ord Ordering.na)
-  .
-
   Variant pf_certify (loc: Loc.t) (th: Thread.t lang): Prop :=
     | pf_certify_failure
         pf e th1 th2
-        (STEPS: rtc (Thread.pf_tau_step (Global.max_reserved (Thread.global th))) th th1)
+        (STEPS: rtc (tau (Thread.step (Global.max_reserved (Thread.global th)) true)) th th1)
         (STEP_FAILURE: Thread.step (Global.max_reserved (Thread.global th)) pf e th1 th2)
         (EVENT_FAILURE: ThreadEvent.get_machine_event e = MachineEvent.failure)
     | pf_certify_fulfill
         pf e th1 th2
         from to val released ord
-        (STEPS: rtc (Thread.pf_tau_step (Global.max_reserved (Thread.global th))) th th1)
+        (STEPS: rtc (tau (Thread.step (Global.max_reserved (Thread.global th)) true)) th th1)
         (STEP_FULFILL: Thread.step (Global.max_reserved (Thread.global th)) pf e th1 th2)
         (EVENT_FULFILL: ThreadEvent.is_writing e = Some (loc, from, to, val, released, ord))
         (TO: Time.lt (Memory.max_ts loc (Global.memory (Thread.global th1))) to)
         (ORD: Ordering.le ord Ordering.na)
   .
 
-  Lemma consistent_certify
+  Variant certify (reserved: OptTimeMap.t) (loc: Loc.t) (th: Thread.t lang): Prop :=
+    | certify_failure
+        pf e th1 th2
+        (STEPS: rtc (pstep (Thread.step_allpf reserved) (fun e => ~ ThreadEvent.is_sc e)) th th1)
+        (STEP_FAILURE: Thread.step reserved pf e th1 th2)
+        (EVENT_FAILURE: ThreadEvent.get_machine_event e = MachineEvent.failure)
+    | certify_fulfill
+        pf e th1 th2
+        from to val released ord
+        (STEPS: rtc (pstep (Thread.step_allpf reserved) (fun e => ~ ThreadEvent.is_sc e)) th th1)
+        (STEP_FULFILL: Thread.step reserved pf e th1 th2)
+        (EVENT_FULFILL: ThreadEvent.is_writing e = Some (loc, from, to, val, released, ord))
+        (TO: Time.lt (Memory.max_ts loc (Global.memory (Thread.global th1))) to)
+        (ORD: Ordering.le ord Ordering.na)
+  .
+
+  Variant non_sc_consistent (th: Thread.t lang): Prop :=
+    | non_sc_consistent_failure
+        pf e th1 th2
+        (STEPS: rtc (pstep (Thread.step_allpf (Global.max_reserved (Thread.global th))) (fun e => ~ ThreadEvent.is_sc e)) th th1)
+        (STEP_FAILURE: Thread.step (Global.max_reserved (Thread.global th)) pf e th1 th2)
+        (EVENT_FAILURE: ThreadEvent.get_machine_event e = MachineEvent.failure)
+    | non_sc_consistent_promises
+        th2
+        (STEPS: rtc (pstep (Thread.step_allpf (Global.max_reserved (Thread.global th))) (fun e => ~ ThreadEvent.is_sc e)) th th2)
+        (PROMISES: Local.promises (Thread.local th2) = BoolMap.bot)
+  .
+
+  Lemma rtc_tau_step_rtc_non_sc_step
+        reserved (th1 th2: Thread.t lang)
+        (STEPS: rtc (Thread.tau_step reserved) th1 th2):
+    exists th2',
+      (<<STEPS1: rtc (pstep (Thread.step_allpf reserved) (fun e => ~ ThreadEvent.is_sc e)) th1 th2'>>) /\
+      ((<<TH2: th2' = th2>>) \/
+       (<<STEPS2: rtc (Thread.tau_step reserved) th2' th2>>) /\
+       (<<PROMISES: Local.promises (Thread.local th2') = BoolMap.bot>>)).
+  Proof.
+    induction STEPS.
+    { esplits; eauto. }
+    inv H. inv TSTEP.
+    destruct (classic (ThreadEvent.is_sc e)).
+    - esplits; [refl|]. right. split.
+      + econs 2; eauto. econs; eauto.
+      + inv STEP; inv STEP0; ss. inv LOCAL. auto.
+    - des.
+      + esplits; [|eauto]. eauto.
+      + esplits; [|eauto]. eauto.
+  Qed.
+
+  Lemma consistent_non_sc_consistent
+        th
+        (CONS: Thread.consistent th):
+    non_sc_consistent th.
+  Proof.
+    inv CONS.
+    - inv FAILURE.
+      exploit rtc_tau_step_rtc_non_sc_step; eauto. i. des.
+      + subst. econs 1; eauto.
+      + econs 2; eauto.
+    - exploit rtc_tau_step_rtc_non_sc_step; eauto. i. des.
+      + subst. econs 2; eauto.
+      + econs 2; eauto.
+  Qed.
+
+  Lemma non_sc_consistent_certify
         th loc
         (LC_WF: Local.wf (Thread.local th) (Thread.global th))
         (GL_WF: Global.wf (Thread.global th))
-        (CONS: Thread.consistent th)
+        (CONS: non_sc_consistent th)
         (PROMISED: Local.promises (Thread.local th) loc = true):
     certify (Global.max_reserved (Thread.global th)) loc th.
   Proof.
     inv CONS.
-    { inv FAILURE. econs 1; eauto. }
+    { econs 1; eauto. }
     remember (Global.max_reserved (Thread.global th)) as reserved.
     clear Heqreserved. revert PROMISED.
     induction STEPS; i.
     { rewrite PROMISES in *. ss. }
     destruct (Local.promises (Thread.local y) loc) eqn:PROMISEDY.
-    { dup H. inv H0. inv TSTEP.
+    { dup H. inv H0. inv STEP.
       exploit Thread.step_future; try exact STEP; eauto. i. des.
       exploit IHSTEPS; eauto. i. inv x1.
       - econs 1; try exact STEP_FAILURE; eauto.
@@ -80,8 +130,8 @@ Section PFCertify.
     }
 
     move PROMISEDY at bottom.
-    inv H. inv TSTEP.
-    inv STEP; inv STEP0; ss; (try congr); (try by inv LOCAL; ss; congr).
+    inv H. inv STEP.
+    inv STEP0; inv STEP; ss; (try congr); (try by inv LOCAL; ss; congr).
     { (* promise *)
       inv LOCAL. inv PROMISE. ss.
       exploit BoolMap.add_le; try exact ADD; eauto. i. congr.
@@ -137,6 +187,154 @@ Section PFCertify.
         (MEMORY: Global.memory (Thread.global th_src) = Global.memory (Thread.global th_tgt))
   .
 
+  Program Instance sim_thread_Equivalence: Equivalence sim_thread.
+  Next Obligation.
+    ii. econs; ss.
+  Qed.
+  Next Obligation.
+    ii. inv H. ss.
+  Qed.
+  Next Obligation.
+    ii. inv H. inv H0. econs; try congr.
+  Qed.
+
+  Lemma sim_thread_internal_step
+        th1_src
+        reserved e th1_tgt th2_tgt
+        (SIM1: sim_thread th1_src th1_tgt)
+        (STEP_TGT: Thread.step reserved false e th1_tgt th2_tgt):
+    sim_thread th1_src th2_tgt.
+  Proof.
+    inv SIM1. inv STEP_TGT. ss. inv STEP.
+    - inv LOCAL. econs; ss.
+      rewrite PROMISES.
+      eauto using Promises.promise_minus.
+    - inv LOCAL. econs; ss.
+      rewrite RESERVES.
+      eauto using Reserves.reserve_minus.
+    - inv LOCAL. econs; ss.
+      rewrite RESERVES.
+      eauto using Reserves.cancel_minus.
+  Qed.
+
+  Lemma sim_is_racy
+        lc_src gl_src lc_tgt gl_tgt
+        loc to ord
+        (TVIEW: Local.tview lc_src = Local.tview lc_tgt)
+        (PROMISES: BoolMap.minus (Global.promises gl_src) (Local.promises lc_src) =
+                   BoolMap.minus (Global.promises gl_tgt) (Local.promises lc_tgt))
+        (MEMORY: Global.memory gl_src = Global.memory gl_tgt)
+        (RACE_TGT: Local.is_racy lc_tgt gl_tgt loc to ord):
+    Local.is_racy lc_src gl_src loc to ord.
+  Proof.
+    inv RACE_TGT.
+    - eapply equal_f in PROMISES.
+      unfold BoolMap.minus in *.
+      rewrite GET, GETP in *. ss.
+      destruct (Global.promises gl_src loc) eqn:GRSV; ss.
+      destruct (Local.promises lc_src loc) eqn:RSV; ss.
+      econs 1; eauto.
+    - rewrite <- TVIEW, <- MEMORY in *. eauto.
+  Qed.
+
+  Lemma sim_thread_program_step
+        (reserved: OptTimeMap.t)
+        th1_src
+        e th1_tgt th2_tgt
+        (RESERVED: forall loc, reserved loc <-> Global.reserves (Thread.global th1_src) loc)
+        (SIM1: sim_thread th1_src th1_tgt)
+        (STEP_TGT: Thread.step reserved true e th1_tgt th2_tgt)
+        (NONSC: ~ ThreadEvent.is_sc e):
+    exists th2_src,
+      (<<STEP_SRC: Thread.step reserved true e th1_src th2_src>>) /\
+      (<<SIM2: sim_thread th2_src th2_tgt>>).
+  Proof.
+    destruct th1_src as [st1_src [tview1_src prm1_src rsv1_src] [sc1_src gprm1_src grsv1_src mem1_src]],
+        th1_tgt as [st1_tgt [tview1_tgt prm1_tgt rsv1_tgt] [sc1_tgt gprm1_tgt grsv1_tgt mem1_tgt]].
+    inv SIM1. ss. subst.
+    inv STEP_TGT. inv STEP; ss.
+    { (* silent *)
+      esplits.
+      - econs; [|econs 1]; eauto.
+      - ss.
+    }
+    { (* read *)
+      inv LOCAL. ss.
+      esplits.
+      - econs; [|econs 2]; eauto.
+      - ss.
+    }
+    { (* write *)
+      inv LOCAL. ss.
+      esplits.
+      - econs; [|econs 3]; eauto.
+        econs; s; eauto. i.
+        exploit NON_RESERVED; eauto. i. des; auto.
+        specialize (RESERVED loc). rewrite GET in *.
+        destruct (grsv1_src loc) eqn:GRSV_SRC; ss; try by intuition.
+        destruct (rsv1_src loc) eqn:RSV_SRC; auto.
+        eapply equal_f in RESERVES.
+        unfold BoolMap.minus in RESERVES.
+        rewrite GRSV_SRC, RSV_SRC, x0 in RESERVES. ss.
+        destruct (grsv1_tgt loc); ss.
+      - econs; ss.
+        rewrite PROMISES.
+        eauto using Promises.fulfill_minus.
+    }
+    { (* update *)
+      inv LOCAL1. inv LOCAL2. ss.
+      esplits.
+      - econs; [|econs 4]; eauto.
+        econs; s; eauto. i.
+        exploit NON_RESERVED; eauto. i. des; auto.
+        specialize (RESERVED loc). rewrite GET0 in *.
+        destruct (grsv1_src loc) eqn:GRSV_SRC; ss; try by intuition.
+        destruct (rsv1_src loc) eqn:RSV_SRC; auto.
+        eapply equal_f in RESERVES.
+        unfold BoolMap.minus in RESERVES.
+        rewrite GRSV_SRC, RSV_SRC, x0 in RESERVES. ss.
+        destruct (grsv1_tgt loc); ss.
+      - econs; ss.
+        rewrite PROMISES.
+        eauto using Promises.fulfill_minus.
+    }
+    { (* fence *)
+      inv LOCAL. ss.
+      esplits.
+      - econs; [|econs 5]; eauto. econs; ss.
+      - ss.
+    }
+    { (* failure *)
+      inv LOCAL. ss.
+      esplits.
+      - econs; [|econs 7]; eauto.
+      - ss.
+    }
+    { (* racy read *)
+      inv LOCAL. ss.
+      esplits.
+      - econs; [|econs 8]; eauto.
+        econs. eapply sim_is_racy; try eapply RACE; ss.
+      - ss.
+    }
+    { (* racy write *)
+      inv LOCAL. ss.
+      esplits.
+      - econs; [|econs 9]; eauto.
+        econs. eapply sim_is_racy; try eapply RACE; ss.
+      - ss.
+    }
+    { (* racy update *)
+      esplits.
+      - econs; [|econs 10]; eauto.
+        inv LOCAL.
+        + econs 1. ss.
+        + econs 2. ss.
+        + econs 3. eapply sim_is_racy; try eapply RACE; ss.
+      - ss.
+    }
+  Qed.
+
   Lemma certify_pf_certify
         th loc
         (LC_WF: Local.wf (Thread.local th) (Thread.global th))
@@ -154,6 +352,8 @@ Section PFCertify.
         (PROMISED: th.(Thread.local).(Local.promises) loc = true):
     pf_certify loc th.
   Proof.
-    eauto using consistent_certify, certify_pf_certify.
+    apply certify_pf_certify; auto.
+    apply non_sc_consistent_certify; auto.
+    apply consistent_non_sc_consistent; auto.
   Qed.
 End PFCertify.
